experiment/Experiment.Steel.Tac.Test.fst
@@ -161,14 +161,14 @@ let test_LCspec (v0 v1 : vprop') (vx0 : int -> vprop')
   : lin_cond_r [v0; v1] (specT int [v0] (fun x -> [vx0 x]))
   = _ by (
     norm_test (); apply (`Mklin_cond_r);
-    build_LCspec test_flags None
+    build_LCspec test_flags dummy_ctx None
   )
 
 let test_LCret (v0 v1 : vprop') (vx0 : int -> vprop')
   : lin_cond_r [v0; v1; vx0 0] (M.Tret int 0 (fun x -> [v1; vx0 x]))
   = _ by (
     norm_test (); apply (`Mklin_cond_r);
-    build_LCret test_flags None
+    build_LCret test_flags dummy_ctx None
   )
 
 let test_LCbind (v0 v1 v2 v3 : vprop') (vx0 vx1 : int -> vprop')
@@ -176,7 +176,7 @@ let test_LCbind (v0 v1 v2 v3 : vprop') (vx0 vx1 : int -> vprop')
                                    (fun x -> specT int [vx0 x; v1] (fun y -> [vx1 y])))
   = _ by (
     norm_test (); apply (`Mklin_cond_r);
-    build_LCbind test_flags None
+    build_LCbind test_flags dummy_ctx None
   )
 
 let test_LCbindP_0 (v0 v1 : vprop') (vx0 : int -> vprop') (wp : pure_wp int)
@@ -184,7 +184,7 @@ let test_LCbindP_0 (v0 v1 : vprop') (vx0 : int -> vprop') (wp : pure_wp int)
         (M.TbindP int int wp (fun x -> specT int [v0] (fun y -> [vx0 y])))
   = _ by (
     norm_test (); apply (`Mklin_cond_r);
-    build_LCbindP test_flags None
+    build_LCbindP test_flags dummy_ctx None
   )
 
 let test_LCbindP_1 (v0 v1 : vprop') (vx0 : int -> vprop') (wp : pure_wp int)
@@ -194,7 +194,7 @@ let test_LCbindP_1 (v0 v1 : vprop') (vx0 : int -> vprop') (wp : pure_wp int)
     norm_test (); apply (`Mklin_cond_r);
     apply (`LV.LCbindP);
     let x = intro () in
-    build_lin_cond test_flags None
+    build_lin_cond test_flags dummy_ctx None
   )
 
 [@@ expect_failure [228]]
@@ -203,7 +203,7 @@ let test_LCbindP_2 (vx0 : int -> vprop') (wp : pure_wp int)
         (M.TbindP int int wp (fun x -> specT int [] (fun y -> [vx0 x])))
   = _ by (
     norm_test (); apply (`Mklin_cond_r);
-    build_LCbindP test_flags None
+    build_LCbindP test_flags dummy_ctx None
   )
 
 
@@ -212,14 +212,14 @@ let test_lin_cond0 (v : int -> vprop') (vx : int -> int -> vprop')
       (M.Tbind int int (specT int [v 0] (fun x -> [v 3; vx 0 x]))
              (fun x -> specT int [vx 0 x; v 1] (fun y -> [vx 1 y])))
       [v 0; v 1; v 2] (fun y -> [v 3; vx 1 y; v 2])
-  = _ by (norm_test (); build_top_lin_cond test_flags)
+  = _ by (norm_test (); build_top_lin_cond test_flags dummy_ctx)
 
 let test_lin_cond1 (v : vprop') (vx : int -> vprop')
   : LV.top_lin_cond
       (M.Tbind int int (M.Tret int 0 (fun x -> [vx x]))
              (fun x -> M.Tret int x (fun x -> [vx x])))
       [v; vx 0] (fun x -> [v; vx x])
-  = _ by (build_top_lin_cond test_flags)
+  = _ by (build_top_lin_cond test_flags dummy_ctx)
 
 /// This example succeeds thanks to the propagation of a production hind ([prd_hint]) which allows to use the top-level
 /// post-condition to infer the dependency on [x] introduced by the [M.Tret].
@@ -227,13 +227,13 @@ let test_lin_cond__ret_hint0 (vx : int -> vprop')
   : LV.top_lin_cond
       (M.Tret int 0 (fun _ -> []))
       [vx 0] (fun x -> [vx x])
-  = _ by (build_top_lin_cond test_flags)
+  = _ by (build_top_lin_cond test_flags dummy_ctx)
 
 let test_lin_cond__ret_hint1 (vx : int -> vprop')
   : LV.top_lin_cond
       (M.Tret int 0 (fun x -> [vx x]))
       [vx 0] (fun x -> [vx x])
-  = _ by (build_top_lin_cond test_flags)
+  = _ by (build_top_lin_cond test_flags dummy_ctx)
 
 [@@ expect_failure [228]]
 let test_lin_cond__ret_hint2 (vx : int -> vprop')
@@ -242,7 +242,7 @@ let test_lin_cond__ret_hint2 (vx : int -> vprop')
          (M.Tret int 0 (fun _ -> []))
          (fun x -> M.Tret int x (fun _ -> [])))
       [vx 0] (fun x -> [vx x])
-  = _ by (build_top_lin_cond test_flags)
+  = _ by (build_top_lin_cond test_flags dummy_ctx)
 
 let test_lin_cond__ret_hint3 (vx : int -> vprop')
   : LV.top_lin_cond
@@ -250,7 +250,7 @@ let test_lin_cond__ret_hint3 (vx : int -> vprop')
          (M.Tret int 0 (fun x -> [vx x]))
          (fun x -> M.Tret int x (fun _ -> [])))
       [vx 0] (fun x -> [vx x])
-  = _ by (build_top_lin_cond test_flags)
+  = _ by (build_top_lin_cond test_flags dummy_ctx)
 
 
 [@@ expect_failure [228]]
@@ -258,7 +258,7 @@ let test_lin_cond__fail0 (v : int -> vprop')
   : LV.top_lin_cond
       (M.Tret int 0 (fun _ -> [v 1]))
       [v 0] (fun _ -> [v 1])
-  = _ by (build_top_lin_cond test_flags)
+  = _ by (build_top_lin_cond test_flags dummy_ctx)
 
 [@@ expect_failure [228]]
 let test_lin_cond__fail1 (vx : int -> vprop')
@@ -266,21 +266,21 @@ let test_lin_cond__fail1 (vx : int -> vprop')
       (M.Tbind int int (specT int [] (fun x -> [vx x]))
              (fun x -> M.Tret int 0 (fun _ -> [])))
       [] (fun x -> [])
-  = _ by (norm_test (); build_top_lin_cond test_flags)
+  = _ by (norm_test (); build_top_lin_cond test_flags dummy_ctx)
 
 
 let test_lin_cond__if_0 (v0 v1 v2 : vprop')
   : LV.top_lin_cond
         (M.Tif _ true (specT int [v0] (fun _ -> [v1])) (specT int [v0] (fun _ -> [v1])))
         [v0; v2] (fun _ -> [v1; v2])
-  = _ by (norm_test (); build_top_lin_cond test_flags)
+  = _ by (norm_test (); build_top_lin_cond test_flags dummy_ctx)
 
 let test_lin_cond__if_1 (v : int -> vprop')
   : LV.top_lin_cond
         (M.Tif _ true (specT int [v 0] (fun _ -> [v 0]))
                       (specT int [v 1] (fun _ -> [v 1])))
         [v 0; v 1; v 2] (fun _ -> [v 0; v 1; v 2])
-  = _ by (norm_test (); build_top_lin_cond test_flags)
+  = _ by (norm_test (); build_top_lin_cond test_flags dummy_ctx)
 
 [@@ expect_failure [228]]
 let test_lin_cond__if_2 (v : int -> vprop')
@@ -288,7 +288,7 @@ let test_lin_cond__if_2 (v : int -> vprop')
         (M.Tif _ true (specT int [v 0] (fun _ -> [v 1]))
                       (specT int []    (fun _ -> [])))
         [v 0] (fun _ -> [v 1])
-  = _ by (norm_test (); build_top_lin_cond test_flags)
+  = _ by (norm_test (); build_top_lin_cond test_flags dummy_ctx)
 
 [@@ expect_failure [228]]
 let test_lin_cond__if_3 (vx : int -> vprop')
@@ -298,7 +298,7 @@ let test_lin_cond__if_3 (vx : int -> vprop')
                         (M.Tret int 0 (fun _ -> [])))
           (fun x -> M.Tret int x (fun _ -> [])))
         [vx 0] (fun x -> [vx x])
-  = _ by (norm_test (); build_top_lin_cond test_flags)
+  = _ by (norm_test (); build_top_lin_cond test_flags dummy_ctx)
 
 let test_lin_cond__if_3 (vx : int -> vprop')
   : LV.top_lin_cond
@@ -307,7 +307,7 @@ let test_lin_cond__if_3 (vx : int -> vprop')
                         (M.Tret int 0 (fun _ -> [])))
           (fun x -> M.Tret int x (fun _ -> [])))
         [vx 0] (fun x -> [vx x])
-  = _ by (norm_test (); build_top_lin_cond test_flags)
+  = _ by (norm_test (); build_top_lin_cond test_flags dummy_ctx)
 
 [@@ expect_failure [228]]
 let test_lin_cond__if_4 (vx : int -> vprop')
@@ -317,4 +317,4 @@ let test_lin_cond__if_4 (vx : int -> vprop')
                         (M.Tret int 0 (fun x -> [vx x])))
           (fun x -> M.Tret int x (fun _ -> [])))
         [vx 0] (fun x -> [vx x])
-  = _ by (norm_test (); build_top_lin_cond test_flags)
+  = _ by (norm_test (); build_top_lin_cond test_flags dummy_ctx)
